wip: Code without proofs

TM/Code/Code.v
@@ -1,259 +1,75 @@
 Require Import TM.Prelim.
 Require Import Coq.Lists.List.
 
-(** * Codeable Class **)
+(** * Codable Class **)
 
-Section Codeable.
 
-  Variable (sigma : finType).
-  Variable (X : Type).
+Generalizable Variables X Y Z sigma sig tau.
 
-  Definition encoding_function := X -> list sigma.
 
-  Class codeable :=
-    mk_codeable
+Section Codable.
+
+  Variable (sig: finType).
+  Variable (X: Type).
+
+  Definition encoding_function := X -> list sig.
+
+  Class codable :=
+    mk_codable
       {
         encode : encoding_function;
-        encode_injective : forall (v1 v2 : X) (r1 r2 : list sigma), encode v1 ++ r1 = encode v2 ++ r2 -> v1 = v2 /\ r1 = r2;
       }.
 
-  Hypothesis codeable_X : codeable.
+  Hypothesis codable_X : codable.
 
-  Lemma encode_injective' : forall v1 v2 : X, encode v1 = encode v2 -> v1 = v2.
-  Proof.
-    intros v1 v2 H.
-    assert (encode v1 ++ [] = encode v2 ++ []) by now rewrite !app_nil_r.
-    now apply encode_injective in H0.
-  Qed.
+End Codable.
+Arguments encode { sig } { X } { _ }.
 
-End Codeable.
-Arguments encode { _ } { _ } { _ }.
 
 Section Encode_Finite.
-  Variable X : finType.
+  (* HACK: [encode true] would not work if we just define [Variable X:finType] *)
+  Context `{fX: finTypeC X}.
 
-  Lemma encode_finite_injective :
-    forall (v1 v2 : X) (r1 r2 : list X),
-      [v1] ++ r1 = [v2] ++ r2 -> v1 = v2 /\ r1 = r2.
-  Proof. firstorder; now inv H. Qed.
+  Global Instance Encode_Finite : codable (FinType X) (FinType X) :=
+    {
+      encode := fun x => [x];
+    }.
 
-  Global Instance Encode_Finite : codeable X X.
-  Proof. apply mk_codeable with (encode := fun x => [x]). apply encode_finite_injective. Defined.
 End Encode_Finite.
 
-Global Instance Encode_Bool : codeable (FinType (EqType bool)) bool := Encode_Finite (FinType (EqType bool)).
+(*
+Global Instance Encode_Bool : codable (FinType (EqType bool)) bool := Encode_Finite (FinType (EqType bool)).
+*)
 
+Compute encode true.
+Compute encode (Fin10: Fin.t 11).
 
-Section RListInduction.
-  Variable X : Type.
-
-  Inductive rlist : list X -> Type :=
-  | rnil  : rlist []
-  | rcons : forall xs x, rlist xs -> rlist (xs ++ [x]).
-
-  Lemma rlist_cons (xs : list X) (x : X) :
-    rlist xs -> rlist (x :: xs).
-  Proof.
-    intros H. induction H.
-    - replace ([x]) with ([] ++ [x]). constructor. constructor. apply app_nil_l.
-    - replace (x :: xs ++ [x0]) with ((x :: xs) ++ [x0]) by reflexivity. now constructor.
-  Qed.
-
-  Lemma rlist_induction : forall xs : list X, rlist xs.
-  Proof.
-    intros xs. induction xs.
-    - constructor.
-    - now apply rlist_cons.
-  Qed.
-
-End RListInduction.
-
-Section DoubleListInduction.
-  Variable (X Y : Type).
-
-  Inductive dlistInd : list X -> list Y -> Prop :=
-  | dlist_nil_nil   : dlistInd nil nil
-  | dlist_nil_cons  : forall y ys, dlistInd nil ys -> dlistInd nil (y :: ys)
-  | dlist_cons_nil  : forall x xs, dlistInd xs nil -> dlistInd (x :: xs) nil
-  | dlist_cons_cons : forall x xs y ys, dlistInd xs ys -> dlistInd (x :: xs) ys -> dlistInd xs (y :: ys) -> dlistInd (x :: xs) (y :: ys).
-
-  Lemma doublelistinduction_xs_nil xs : dlistInd xs nil.
-  Proof. induction xs; now constructor. Qed.
-
-  Lemma doublelistinduction_nil_ys ys : dlistInd nil ys.
-  Proof. induction ys; now constructor. Qed.
-
-  Lemma doubleListInduction xs ys : dlistInd xs ys.
-  Proof.
-    revert ys. induction xs; intros ys.
-    - apply doublelistinduction_nil_ys.
-    - destruct ys.
-      + constructor. apply doublelistinduction_xs_nil.
-      + constructor; auto. induction ys; constructor; auto.
-  Qed.
-
-End DoubleListInduction.
-
-Section Map_Retract.
-  Variable (X : Type).
-  Variable (sig tau : finType).
-  Hypothesis (code_sig : codeable sig X).
-  Variable (f : sig -> tau) (g : tau -> option sig).
-  Hypothesis (inj : retract f g).
-
-  Lemma map_map_app_eq_None_None (ss1 ss2 : list sig) (t1 t2 : tau) (ts1 ts2 : list tau) :
-    g t1 = None -> g t2 = None ->
-    map f ss1 ++ [t1] ++ ts1 = map f ss2 ++ [t2] ++ ts2 ->
-    map f ss1 = map f ss2 /\ t1 = t2 /\ ts1 = ts2.
-  Proof.
-    intros H1 H2 H. induction (doubleListInduction ss1 ss2); cbn in *.
-    - now inv H.
-    - exfalso. inv H. clear H2 ys d IHd. enough (g (f y) = Some y) by congruence. now retract_adjoint.
-    - exfalso. inv H. clear H1 xs d IHd. enough (g (f x) = Some x) by congruence. now retract_adjoint.
-    - inv H.
-      enough (map f xs = map f ys /\ t1 = t2 /\ ts1 = ts2) as (HE1&HE2).
-      { split; now f_equal. }
-      now apply IHd1.
-  Qed.
-
-  Lemma map_map_app_eq (ss1 ss2 : list sig) (ts : list tau) :
-    map f ss1 = map f ss2 ++ ts ->
-    exists ss3, map f ss1 = map f ss2 ++ map f ss3.
-  Proof.
-    revert ss2 ts. induction ss1; intros ss2 ts H; cbn in *.
-    - symmetry in H. apply appendNil in H as (H&->). apply map_eq_nil in H as ->. exists nil. reflexivity.
-    - destruct ss2; cbn in *.
-      + destruct ts.
-        * congruence.
-        * exists (a :: ss1). reflexivity.
-      + inv H. specialize (IHss1 _ _ H2) as (ss3&IH). eexists. f_equal. rewrite IH. f_equal.
-  Qed.
-
-  Lemma map_app_eq_nil_None (ss1 ss2 : list sig) (t : tau) (ts : list tau) :
-    g t = None -> map f ss1 <> map f ss2 ++ [t] ++ ts.
-  Proof.
-    intros H C.
-    assert (forall x, x el (map f ss1) -> g x <> None) as Contra.
-    {
-      intros x (x'&<-&_) % in_map_iff. retract_adjoint. congruence.
-    }
-    rewrite C in Contra. apply (Contra t); auto.
-  Qed.
-
-End Map_Retract.
 
 Section Encode_Map.
   Variable (X : Type).
   Variable (sig tau : finType).
-  Hypothesis (code_sig : codeable sig X).
-  Variable (f : sig -> tau) (g : tau -> option sig).
+  Hypothesis (code_sig : codable sig X).
+  Variable (f : sig -> tau).
 
-  (*
-   * We actually do not need the retract to be tight, since sig and tau are finite.
-   * If there is a retract for f and g, Coq will automaticly find a function g' : tau -> option sig,
-   * such that (f, g') is a tight retract.
-   *)
-  Hypothesis (inj : tight_retract f g).
-
-  Lemma encode_map_injective':
-    forall (v1 v2 : X) (r1 r2 : list sig) (R1 R2 : list tau),
-      map f (encode v1 ++ r1) ++ R1 = map f (encode v2 ++ r2) ++ R2 -> v1 = v2 /\ map f r1 ++ R1 = map f r2 ++ R2.
-  Proof.
-    intros. revert r1 r2 H.
-    induction (doubleListInduction R1 R2); intros r1 r2 H; cbn in *.
-    - rewrite !app_nil_r in H. apply map_injective in H. apply encode_injective in H. intuition. congruence. auto_inj.
-    - destruct (g y) eqn:E.
-      + eapply tretract_g_inv' in E; auto_inj; subst.
-        replace (f e :: ys) with (map f [e] ++ ys) in H by reflexivity.
-        rewrite app_assoc in H. rewrite <- map_app in H. rewrite <- app_assoc in H.
-        pose proof (IHd _ _ H) as (->&IH). rewrite !app_nil_r in *.
-        rewrite map_app in IH. rewrite <- app_assoc in IH. auto.
-      + rewrite !app_nil_r in *. exfalso. replace (y :: ys) with ([y] ++ ys) in H by reflexivity. eapply map_app_eq_nil_None; auto_inj.
-    - destruct (g x) eqn:E.
-      + eapply tretract_g_inv' in E; auto_inj; subst.
-        replace (f e :: xs) with (map f [e] ++ xs) in H by reflexivity.
-        rewrite app_assoc in H. rewrite <- map_app in H. rewrite <- app_assoc in H.
-        pose proof (IHd _ _ H) as (->&IH). rewrite !app_nil_r in *.
-        rewrite map_app in IH. rewrite <- app_assoc in IH. auto.
-      + rewrite !app_nil_r in *. exfalso. replace (x :: xs) with ([x] ++ xs) in H by reflexivity. eapply map_app_eq_nil_None; auto_inj.
-    - destruct (g x) eqn:E1, (g y) eqn:E2.
-      + eapply tretract_g_inv' in E1; auto_inj; subst. eapply tretract_g_inv' in E2; auto_inj; subst.
-        replace (f e  :: xs) with (map f [e ] ++ xs) in H by reflexivity.
-        replace (f e0 :: ys) with (map f [e0] ++ ys) in H by reflexivity.
-        rewrite app_assoc in H. rewrite <- map_app in H. rewrite <- app_assoc in H. symmetry in H.
-        rewrite app_assoc in H. rewrite <- map_app in H. rewrite <- app_assoc in H. symmetry in H.
-        pose proof (IHd1 _ _ H) as (->&IH). rewrite !map_app in IH. rewrite <- !app_assoc in IH. split; auto.
-      + eapply tretract_g_inv' in E1; auto_inj; subst.
-        replace (f e  :: xs) with (map f [e ] ++ xs) in H by reflexivity.
-        rewrite app_assoc in H. rewrite <- map_app in H. rewrite <- app_assoc in H.
-        pose proof (IHd3 _ _ H) as (->&IH). rewrite !map_app in IH. rewrite <- !app_assoc in IH. split; auto.
-      + eapply tretract_g_inv' in E2; auto_inj; subst.
-        replace (f e  :: ys) with (map f [e ] ++ ys) in H by reflexivity.
-        rewrite app_assoc in H. rewrite <- map_app in H. rewrite <- app_assoc in H.
-        pose proof (IHd2 _ _ H) as (->&IH). rewrite !map_app in IH. rewrite <- !app_assoc in IH. split; auto.
-      + replace (x :: xs) with ([x] ++ xs) in H by reflexivity. replace (y :: ys) with ([y] ++ ys) in H by reflexivity.
-        pose proof (map_map_app_eq_None_None ltac:(auto_inj) E1 E2 H) as (L&->&->). apply map_injective in L.
-        now apply encode_injective in L as (->&->). auto_inj.
-  Qed.
-
-  Lemma encode_map_injective :
-    forall (v1 v2 : X) (r1 r2 : list tau),
-      map f (encode v1) ++ r1 = map f (encode v2) ++ r2 -> v1 = v2 /\ r1 = r2.
-  Proof.
-    intros. pose proof (@encode_map_injective' v1 v2 nil nil r1 r2) as L. cbn in L. rewrite !app_nil_r in L. auto.
-  Qed.
-
-  Global Instance Encode_Map : codeable tau X.
-  Proof.
-    apply mk_codeable with (encode := fun x => map f (encode (codeable := code_sig) x)).
-    now apply encode_map_injective.
-  Defined.
+  Global Instance Encode_Map : codable tau X :=
+    {
+      encode x := map f (encode x);
+    }.
   
 End Encode_Map.
-
-(* Without the requirement that (f,g) is a tight retract. *)
-Section Encode_Map'.
-  Variable (X : Type).
-  Variable (sig tau : finType).
-  Hypothesis (code_sig : codeable sig X).
-  Variable (f : sig -> tau) (g : tau -> option sig).
-  Hypothesis (inj : retract f g).
-  Definition Encode_Map' : codeable tau X.
-  Proof. eapply Encode_Map. eapply code_sig. eapply make_tight_retract. Defined.
-End Encode_Map'.
-
-  
-(* TODO: Injectivity of the X coding is enough. *)
-Section Stop.
-
-  Variable X : Type.
-  Variable sig : finType.
-  (*
-  Variable enc : encoding_function sig X.
-  Hypothesis enc_injective : forall x y : X, enc x = enc y -> x = y.
-  *)
-  Hypothesis (code_X : codeable sig X).
-
-  Definition encode_stop (x : X) : list (option sig) :=
-    encode (codeable := Encode_Map (tau := FinType (EqType (option sig))) code_X (@retract_option _)) x ++ [None].
-
-  Lemma encode_stop_injective :
-    forall (v1 v2 : X) (r1 r2 : list finType_CS),
-      encode_stop v1 ++ r1 = encode_stop v2 ++ r2 -> v1 = v2 /\ r1 = r2.
-  Proof.
-    intros. unfold encode_stop in H. cbn in *. rewrite <- !app_assoc in H.
-    eapply (encode_injective (codeable := Encode_Map code_X (@retract_option _))) in H as [H1 H2]. now (inv H1; inv H2).
-  Qed.
-  
-  Instance Encode_Stop : codeable (FinType (EqType (option sig))) X := mk_codeable encode_stop_injective.
-  
-End Stop.
 
 
 Section Encode_Sum.
   Variable (X Y : Type).
   Variable (sig tau : finType).
-  Hypothesis (code_X : codeable sig X) (code_Y : codeable tau Y).
+  Hypothesis (cX : codable sig X) (cY : codable tau Y).
+
+  Global Instance Encode_Sum : codable (FinType(EqType(bool+(sig+tau)))) (X+Y) :=
+    {
+      encode s := match s with
+                  | inl x => inl true :: Encode_Map
+
+  
 
 
   Global Instance retract_r_l : TRetract sig (bool + (sig + tau)) := Build_TRetract (tretract_compose _ _).
@@ -275,16 +91,16 @@ Section Encode_Sum.
     - eapply encode_map_injective in H1 as (->&->). tauto. apply retract_r_r.
   Qed.
 
-  Global Instance Encode_Sum : codeable (FinType (EqType (bool + (sig + tau)))) (X + Y) := mk_codeable encode_sum_injective.
+  Global Instance Encode_Sum : codable (FinType (EqType (bool + (sig + tau)))) (X + Y) := mk_codable encode_sum_injective.
 End Encode_Sum.
 
 
 Section Encode_Pair.
   Variable (X Y : Type) (sig : finType).
-  Hypothesis (code_X : codeable sig X) (code_Y : codeable sig Y).
+  Hypothesis (code_X : codable sig X) (code_Y : codable sig Y).
 
   Definition encode_pair (v : X * Y) : list sig.
-  Proof. destruct v as (a,b). apply (encode (codeable := code_X) a ++ encode (codeable := code_Y) b). Defined.
+  Proof. destruct v as (a,b). apply (encode (codable := code_X) a ++ encode (codable := code_Y) b). Defined.
 
   Lemma encode_pair_injective :
     forall (v1 v2 : X * Y) (r1 r2 : list sig), encode_pair v1 ++ r1 = encode_pair v2 ++ r2 -> v1 = v2 /\ r1 = r2.
@@ -293,15 +109,15 @@ Section Encode_Pair.
     apply encode_injective in H as (->&H). apply encode_injective in H as (->&->). auto.
   Qed.
 
-  Global Instance Encode_Pair : codeable sig (X * Y) := mk_codeable encode_pair_injective.
+  Global Instance Encode_Pair : codable sig (X * Y) := mk_codable encode_pair_injective.
 End Encode_Pair.
 
 Section Encode_Pair'.
   Variable (X Y : Type) (sig tau : finType).
 
-  Hypothesis (code_X : codeable sig X) (code_Y : codeable tau Y).
+  Hypothesis (code_X : codable sig X) (code_Y : codable tau Y).
 
-  Global Instance Encode_Pair' : codeable (FinType (EqType (sig + tau)%type)) (X * Y).
+  Global Instance Encode_Pair' : codable (FinType (EqType (sig + tau)%type)) (X * Y).
   Proof.
     apply Encode_Pair; apply (Encode_Map _ _).
   Defined.
@@ -316,7 +132,7 @@ Section Encode_Unit.
     forall (v1 v2 : unit) (r1 r2 : list (FinType (EqType Empty_set))), encode_unit v1 ++ r1 = encode_unit v2 ++ r2 -> v1 = v2 /\ r1 = r2.
   Proof. intros () () r1 r2. auto. Qed.
 
-  Global Instance Encode_Unit : codeable (FinType (EqType Empty_set)) unit := mk_codeable encode_unit_injective.
+  Global Instance Encode_Unit : codable (FinType (EqType Empty_set)) unit := mk_codable encode_unit_injective.
 
 End Encode_Unit.
 
@@ -327,16 +143,16 @@ Section Encode_Empt.
     forall (v1 v2 : Empty_set) (r1 r2 : list (FinType (EqType Empty_set))), encode_empty v1 ++ r1 = encode_empty v2 ++ r2 -> v1 = v2 /\ r1 = r2.
   Proof. intros v1. destruct v1. Qed.
     
-  Global Instance I_empty : codeable (FinType (EqType Empty_set)) Empty_set := mk_codeable encode_empty_injective.
+  Global Instance I_empty : codable (FinType (EqType Empty_set)) Empty_set := mk_codable encode_empty_injective.
 End Encode_Empt.
 
 Section Encode_Cast.
   Variable sig : finType.
   Variable (X Y : Type) (f : Y -> X).
-  Hypothesis (codeX : codeable sig X).
+  Hypothesis (codeX : codable sig X).
   Hypothesis (inj : injective f).
 
-  Lemma Encode_Cast : codeable sig Y.
+  Lemma Encode_Cast : codable sig Y.
   Proof.
     esplit with (encode := fun y => encode (f y)).
     - intros v1 v2 r1 r2 H. apply encode_injective in H as (H&->). split; eauto.
@@ -344,7 +160,7 @@ Section Encode_Cast.
 
 End Encode_Cast.
 
-Lemma Encode_Option' (X : Type) (sig : finType) : codeable sig X -> codeable (FinType (EqType (bool + (sig + Empty_set)))) (option X).
+Lemma Encode_Option' (X : Type) (sig : finType) : codable sig X -> codable (FinType (EqType (bool + (sig + Empty_set)))) (option X).
 Proof.
   intros H. eapply Encode_Cast. eapply Encode_Sum.
   - apply H.
@@ -355,7 +171,7 @@ Proof.
 Defined.
 
 (* Eleminate the Empty_set from above *)
-Global Instance Encode_Option (X : Type) (sig : finType) : codeable sig X -> codeable (FinType (EqType (bool + sig))) (option X).
+Global Instance Encode_Option (X : Type) (sig : finType) : codable sig X -> codable (FinType (EqType (bool + sig))) (option X).
 Proof.
   intros H. eapply Encode_Map. eapply Encode_Option'; auto. eapply inversion_retract. 
   (* (* Just for cosmetics *) Unshelve. all: unfold finType_CS. 2-3: cbn; shelve. Show Existentials. *)
@@ -367,12 +183,12 @@ Defined.
 
 Section Encode_List.
   Variable sig: finType.
-  Variable (X : Type) (code_X : codeable sig X).
+  Variable (X : Type) (code_X : codable sig X).
 
   Fixpoint encode_list (xs : list X) : list (bool + sig) :=
     match xs with
     | nil => [inl false]
-    | x :: xs' => inl true :: encode (codeable := Encode_Map code_X (@retract_inr _ _)) x ++ encode_list xs'
+    | x :: xs' => inl true :: encode (codable := Encode_Map code_X (@retract_inr _ _)) x ++ encode_list xs'
     end.
 
   Lemma encode_injective_list :
@@ -386,7 +202,7 @@ Section Encode_List.
         eapply encode_map_injective in H1 as (->&H1). now specialize (IH _ _ _ H1) as (->&->). apply retract_inr.
   Qed.
 
-  Global Instance Encode_List : codeable (FinType (EqType (bool + sig))) (list X) := mk_codeable encode_injective_list.
+  Global Instance Encode_List : codable (FinType (EqType (bool + sig))) (list X) := mk_codable encode_injective_list.
 
 End Encode_List.
 
@@ -402,7 +218,7 @@ Section Encode_Nat.
     - cbn in *. destruct m; cbn in *. congruence. f_equal. apply IHn. congruence.
   Qed.
 
-  Global Instance Encode_Nat : codeable (FinType (EqType bool)) nat.
+  Global Instance Encode_Nat : codable (FinType (EqType bool)) nat.
   Proof.
     eapply Encode_Map.
     - eapply Encode_Cast.
@@ -432,7 +248,7 @@ Section Encode_Fin'.
     hnf. intros x1 x2. apply fin_to_nat_injective.
   Qed.
 
-  Local Instance Encode_Fin' : codeable (FinType (EqType bool)) (Fin.t n).
+  Local Instance Encode_Fin' : codable (FinType (EqType bool)) (Fin.t n).
   Proof.
     eapply Encode_Cast; [ | eapply cast_Fin ]. apply Encode_Nat.
   Defined.
@@ -466,7 +282,7 @@ Check encode (X := list (FinType (EqType move))).
 Compute encode (X := list (FinType (EqType move))) [L; N; R].
 
 Compute encode (X := FinType (EqType (Fin.t 10))) (Fin.FS (Fin.FS (Fin.FS (Fin.F1)))).
-Compute encode (codeable := Encode_Fin' 10) (Fin.FS (Fin.FS (Fin.FS (Fin.F1)))).
+Compute encode (codable := Encode_Fin' 10) (Fin.FS (Fin.FS (Fin.FS (Fin.F1)))).
 
 Check Encode_Pair' (Encode_List (Encode_Unit)) Encode_Unit.
 
